\begin{lemma}
  Let $\beta,\beta'\in\NN\setminus\{0\}$ and $c_1,\dots,c_\ell \in \ZZ$ such that $|c_i|\leq\beta'$ then
  \[
    2\cdot\Pr[b_i \gets \bin : \Bigl|\sum_{i=1}^\ell b_i\Bigr| > \beta] \geq \Pr[b_i \gets \bin : \Bigl|\sum_{i=1}^\ell b_i c_i\Bigr| > \beta'\beta]
  \]
\end{lemma}
\begin{proof}
  For all $1\leq i \leq \ell$, let $\tilde{c}_i = \beta' - c_i$.
  It holds that
  \begin{align*}
    &\Pr[b_i \gets \bin : \beta'\sum_{i=1}^\ell b_i > \beta'\beta]\\
    =&\Pr[b_i \gets \bin : \sum_{i=1}^\ell b_i (c_i+\tilde{c}_i) > \beta'\beta]\\
    =&\Pr[b_i \gets \bin : \sum_{i=1}^\ell b_i c_i + \sum_{i=1}^\ell b_i \tilde{c}_i > \beta'\beta]\\
    \geq&\Pr[b_i \gets \bin : \sum_{i=1}^\ell b_i c_i + \sum_{i=1}^\ell b_i \tilde{c}_i > \beta'\beta \mid \sum_{i=1}^\ell b_i \tilde{c}_i \geq 0] \cdot \Pr[b_i \gets \bin : \sum_{i=1}^\ell b_i \tilde{c}_i \geq 0]\\
    \geq& \Pr[b_i \gets \bin : \sum_{i=1}^\ell b_i c_i > \beta'\beta]\cdot \frac{1}{2}
  \end{align*}
  where the last inequality follows because for any positive $\sum_{i=1}^\ell b_i \tilde{c}_i$ the total sum and therefore the probability of exceeding any bound can only increase and because the distribution of $\sum_{i=1}^\ell b_i \tilde{c}_i$ is both symmetric and centered at $0$.
  Following the equivalent reasoning it also holds that
  \begin{align*}
    &\Pr[b_i \gets \bin : \beta'\sum_{i=1}^\ell b_i < -\beta'\beta]\\
    =&\Pr[b_i \gets \bin : \sum_{i=1}^\ell b_i (c_i+\tilde{c}_i) < -\beta'\beta]\\
    =&\Pr[b_i \gets \bin : \sum_{i=1}^\ell b_i c_i + \sum_{i=1}^\ell b_i \tilde{c}_i < -\beta'\beta]\\
    \geq&\Pr[b_i \gets \bin : \sum_{i=1}^\ell b_i c_i + \sum_{i=1}^\ell b_i \tilde{c}_i < \beta'\beta \mid \sum_{i=1}^\ell b_i \tilde{c}_i \leq 0] \cdot \Pr[b_i \gets \bin : \sum_{i=1}^\ell b_i \tilde{c}_i \leq 0]\\
    \geq& \Pr[b_i \gets \bin : \sum_{i=1}^\ell b_i c_i < -\beta'\beta]\cdot \frac{1}{2}.
  \end{align*}
  
  Using these two bounds we can then conclude that
  \begin{align*}
    &2\cdot\Pr[b_i \gets \bin : \Bigl|\sum_{i=1}^\ell b_i\Bigr| > \beta]\\
    =&2\cdot\Pr[b_i \gets \bin : \beta'\Bigl|\sum_{i=1}^\ell b_i\Bigr| > \beta'\beta]\\
    \geq&2\cdot(\Pr[b_i \gets \bin : \beta'\sum_{i=1}^\ell b_i > \beta'\beta] + \Pr[b_i \gets \bin : \beta'\sum_{i=1}^\ell b_i < -\beta'\beta])
    \geq \Pr[b_i \gets \bin : \sum_{i=1}^\ell b_i c_i > \beta'\beta]+\Pr[b_i \gets \bin : \sum_{i=1}^\ell b_i c_i < -\beta'\beta]
    = \Pr[b_i \gets \bin : \Bigl|\sum_{i=1}^\ell b_i c_i\Bigr| > \beta'\beta]
  \end{align*}
  where the last equality holds, because $\beta'\beta\neq 0$ and the sum cannot be both positive and negative at the same time.\qed
\end{proof}
